

## Contents

Artin 2.1.5 Consequences of an equation .....	2
Artin 2.1.7 Proving that a given binary op is associative .....	3
Artin 2.2.1 A cyclic matrix group .....	4
Artin 2.2.15 Uniqueness of identity and inverses in subgroups .....	5
Artin 2.2.20(a) The order of products in abelian groups .....	6

### **Artin 2.1.5 Consequences of an equation**

We are given that  $xyz = 1$  in some group  $G$ . So

$$yz = x^{-1}$$

and therefore

$$yzx = 1.$$

But it is not necessarily the case that  $yxz = 1$ . We know  $xy = z^{-1}$  but we don't know that this group is abelian.

### **Artin 2.1.7 Proving that a given binary op is associative**

Given the law of composition

$$ab = a,$$

we must prove that

$$(ab)c = a(bc).$$

The LHS becomes

$$(a)c = ac = a$$

while the RHS becomes

$$a(b) = ab = a$$

so it is proved.

### Artin 2.2.1 A cyclic matrix group

The elements of the cyclic group generated by

$$\begin{bmatrix} 1 & 1 \\ -1 & 0 \end{bmatrix}$$

are its powers:

$$\begin{bmatrix} 1 & 1 \\ -1 & 0 \end{bmatrix}, \begin{bmatrix} 0 & 1 \\ -1 & -1 \end{bmatrix}, \begin{bmatrix} -1 & 0 \\ 0 & -1 \end{bmatrix}, \begin{bmatrix} -1 & -1 \\ 1 & 0 \end{bmatrix}, \begin{bmatrix} 0 & -1 \\ 1 & 1 \end{bmatrix}, \begin{bmatrix} 1 & 0 \\ 0 & 1 \end{bmatrix}.$$

So it's a cyclic group of order 6, isomorphic to the integers modulo 6.

Note that  $A^3 = -I$ , so  $A^6 = I$  is immediate and it's easy to get  $A^4 = -A$  and  $A^5 = -A^2$  from previously computed powers.

## Artin 2.2.15 Uniqueness of identity and inverses in subgroups

(a)

Let  $e_H$  be the identity in  $H$ . Then

$$e_H e_H = e_H$$

but since the operation is inherited from  $G$  we may multiply by  $e_H^{-1}$  in  $G$ :

$$e_H^{-1} e_H e_H = e_H^{-1} e_H$$

to get

$$e_G e_H = e_G,$$

that is,

$$e_H = e_G.$$

(b)

Let  $a^{-H}$  be the inverse in  $H$  and  $a^{-G}$  be the inverse in  $G$ . Then in  $H$  we have

$$a a^{-H} = 1$$

but this equation holds in  $G$  as well we may multiply on the left by  $a^{-G}$  in  $G$  to get

$$a^{-G} a a^{-H} = a^{-G}$$

where the first two factors on the left multiply in  $G$  to give the identity, so

$$a^{-H} = a^{-G}.$$

### Artin 2.2.20(a) The order of products in abelian groups

Let  $a, b$  be elements of an abelian group of orders  $m, n$  respectively. Then if  $l = \text{lcm}(m, n)$ , we see that

$$(ab)^l = a^l b^l = (a^m)^{\frac{l}{m}} (b^n)^{\frac{l}{n}} = 1$$

where all exponents are integers since  $l$  is a multiple of both  $m$  and  $n$ .

But for any element  $x$ , we know that  $x^y = 1$  implies that its order divides  $y$ . So  $\text{ord}(ab) \mid \text{lcm}(m, n)$ .

(Note that this is NOT a consequence of Lagrange's Theorem.

Here's an incorrect argument: the powers of  $x$  from 0 to  $y$  (with potential repeat elements) form a group  $G$ , and the powers of  $x$  from 0 to  $\text{ord}(a)$  form a group  $H$ , but the order is the smallest number with this property, so all the elements of  $H$  are contained in  $G$ , so  $H$  is a subgroup of  $G$ , so  $\text{ord}(H) \mid \text{ord}(G)$ .

The problem is the repeat elements. For this argument to work,  $\text{ord}(G) = y$ , but in fact  $G$  is the same group as  $H$ , so  $\text{ord}(G) = \text{ord}(x)$  and we can't conclude from this argument that  $\text{ord}(x) \mid y$ .)